# Answers to Problem Set IV

*Prepared by*
Christian Y. Cahig

# Problem I

Find the solution to the following differential equation:

$$
\left(
D^{3} - D
\right)
y
= 4 e^{-x} + 3 e^{2x}
$$ (1.0)

Neglecting the right-hand side of (1.0)
gives a homogeneous ODE
whose characteristic equation (in $\lambda$) is
$\lambda^{3} - \lambda = 0$&mdash;that is,
the characteristic roots are
$-1,0,1$.
Hence, the homogeneous solution is the superposition of basis functions
$e^{-x}$, $e^{0x}$, and $e^{x}$:

$$
y_{\textsf{h}}
=
C_{1} e^{-x} + C_{2} e^{0x} + C_{3} e^{x}
=
C_{1} e^{-x} + C_{2} + C_{3} e^{x}
$$ (1.1)
where $C_{1}$, $C_{2}$, and $C_{3}$ are constants.

Inspecting the right-hand side of (1.0),
we can deduce that
$e^{-x}$ and $e^{2x}$
also are basis functions for the general solution.
However, $e^{-x}$ is already "subscribed" to $y_{\textsf{h}}$,
and must therefore be treated as a "repeating" basis.
The particular solution is then the superposition of basis functions
$x e^{-x}$ and $e^{2x}$:

$$
y_{\textsf{p}}
=
C_{4} x e^{-x}
+
C_{5} e^{2x}
$$
where $C_{4}$ and $C_{5}$ are constants.
Differentiating $y_{\textsf{p}}$
successively with respect to $x$,

$$
D y_{\textsf{p}} = y_{\textsf{p}}^{\prime}
=
C_{4} e^{-x} - C_{4} x e^{-x} + 2 C_{5} e^{2x}
$$
$$
D^{3} y_{\textsf{p}} = y_{\textsf{p}}^{\prime \prime \prime}
=
3 C_{4} e^{-x} - C_{4} x e^{-x} + 8 C_{5} e^{2x}
$$
and substituting onto (1.0) will eventually give

$$
2 C_{4} e^{-x} + 6 C_{5} e^{2x}
=
4 e^{-x} + 3 e^{2x}
\quad \Longrightarrow \quad
C_{4} = 2, \quad C_{5} = 0.5
$$
Hence, the particular solution is

$$
y_{\textsf{p}} = 2 x e^{-x} + 0.5 e^{2x}
$$ (1.2)

Therefore, the general solution to (1.0)
is the superposition of
$y_{\textsf{h}}$ and $y_{\textsf{p}}$:

$$
y
=
y_{\textsf{h}} + y_{\textsf{p}}
=
C_{1} e^{-x} + C_{2} + C_{3} e^{x}
+
2 x e^{-x} + 0.5 e^{2x}
$$ (1.3)
where $C_{1}$, $C_{2}$, and $C_{3}$ are constants.

# Problem II

Find the solution to the following differential equation:

$$
\left(
D^{3} - 2 D^{2} + D
\right)
y
=
x
$$ (2.0)

Neglecting the right-hand side of (2.0)
gives a homogeneous ODE
whose characteristic equation (in $\lambda$) is
$\lambda^{3} - 2 \lambda^{2} + \lambda = 0$&mdash;that is,
the characteristic roots are
$0$ and $1$,
the latter having a multiplicity of two.
Hence, the homogeneous solution is the superposition of basis functions
$e^{0x}$, $e^{x}$, and $x e^{x}$:

$$
y_{\textsf{h}}
=
C_{1} e^{0x} + C_{2} e^{x} + C_{3} x e^{x}
=
C_{1} + C_{2} e^{x} + C_{3} x e^{x}
$$ (2.1)
where $C_{1}$, $C_{2}$, and $C_{3}$ are constants.

Inspecting the right-hand side of (2.0),
we can deduce that the particular solution is of the form
$C_{4} x + C_{5}$,
where $C_{4}$ and $C_{5}$ are constants.
However, the constant function $C_{5}$ is already
"subscribed" to $y_{\textsf{h}}$,
and is essentially a "repeat" of the $C_{1}$ term.
The particular solution is then the superposition of basis functions
$x^{2}$ and $x$:

$$
y_{\textsf{p}}
=
C_{4} x^{2} + C_{5} x
$$
Differentiating $y_{\textsf{p}}$
successively with respect to $x$

$$
D y_{\textsf{p}} = y_{\textsf{p}}^{\prime}
=
2 C_{4} x + C_{5}
$$
$$
D^{2} y_{\textsf{p}} = y_{\textsf{p}}^{\prime \prime}
=
2 C_{4}
$$
$$
D^{3} y_{\textsf{p}} = y_{\textsf{p}}^{\prime \prime \prime}
=
0
$$
and substituting onto (2.0) will eventually give

$$
2 C_{4} x + C_{5} - 4 C_{4} = x
\quad \Longrightarrow \quad
C_{4} = 0.5, \quad C_{5} = 2
$$
Hence, the particular solution is

$$
y_{\textsf{p}} = 0.5 x^{2} + 2 x
$$ (2.2)

Therefore, the general solution to (2.0)
is the superposition of
$y_{\textsf{h}}$ and $y_{\textsf{p}}$:

$$
y
=
y_{\textsf{h}} + y_{\textsf{p}}
=
C_{1} + C_{2} e^{x} + C_{3} x e^{x}
+
0.5 x^{2} + 2 x
$$ (1.3)
where $C_{1}$, $C_{2}$, and $C_{3}$ are constants.

# Problem III

Find the solution to the following differential equation:

$$
\left(
D^{4} + 4 D^{2} + 4
\right)
y
=
- 20
$$ (3.0)

Neglecting the right-hand side of (3.0)
gives a homogeneous ODE whose characteristic equation
(in $\lambda$) is
$\lambda^{4} + 3 \lambda^{2} + 4 = 0$.
This corresponds to the complex conjugate roots
$\plusmn \sqrt{2} i$,
each having a multiplicity of two.
This means that the homogeneous solution is
the superposition of the basis functions
$\cos \left(\sqrt{2} x\right)$,
$\sin \left(\sqrt{2} x\right)$,
$x \cos \left(\sqrt{2} x\right)$,
and
$x \sin \left(\sqrt{2} x\right)$:

$$
y_{\textsf{h}} =
C_{1} \cos \left(\sqrt{2} x\right)
+
C_{2} \sin \left(\sqrt{2} x\right)
+
C_{3} x \cos \left(\sqrt{2} x\right)
+
C_{4} x \sin \left(\sqrt{2} x\right)
$$ (3.1)
where $C_{1}$, $C_{2}$, $C_{3}$, and $C_{4}$ are constants.

Inspecting the right-hand side of (3.0),
we can deduce that the particular solution
is a constant $C_{5}$.
Differentiating and substituting to (3.0)
will yield

$$
4 C_{5} = -20
\quad \Longrightarrow \quad
C_{5} = -5
$$
Hence, the particular solution is

$$
y_{\textsf{p}} = - 5
$$ (3.2)

Therefore, the general solution to (3.0)
is the superposition of $y_{\textsf{h}}$ and $y_{\textsf{p}}$:

$$
y
=
y_{\textsf{h}} + y_{\textsf{p}}
=
C_{1} \cos \left(\sqrt{2} x\right)
+
C_{2} \sin \left(\sqrt{2} x\right)
+
C_{3} x \cos \left(\sqrt{2} x\right)
+
C_{4} x \sin \left(\sqrt{2} x\right)
- 5
$$ (3.3)
where $C_{1}$, $C_{2}$, $C_{3}$, and $C_{4}$ are constants.

# Problem IV

A spring is such that
a 2-lb weight stretches it 6 in.
An impressed force of
$0.25 \sin \left(8t\right)$
(lb)
and
a resisting force numerically equal to
the velocity at any instant
are both acting on the spring.
The weight starts 3 in below equilibrium point
with an imparted upward velocity of
3 ft/s.
Find the equation of motion.

Let us first lay down some assumptions and conventions.
We take the spring to be always vertically oriented.
The upper end is fixed,
while the lower end is attached
to the 2-lb weight assumed to be in the form of a point mass $m$.
The instantaneous vertical motion of this mass
is what we seek to describe mathematically.
Let $y$ be the vertical position (in ft) of the mass,
where $y = 0$ corresponds to the equilibrium point
(*i.e.*, when the mass-spring system hangs freely).
We assume $y > 0$ when the mass is above the equilibrium point.

At any $y$, the mass experiences four forces all measured in lb:
the weight $F_{\textsf{m}} = mg = 2$
(where $g = 32.17$ ft/s$^{2}$
is the acceleration due to gravity),
the periodic driving force
$F_{\textsf{d}} = 0.25 \sin \left(8t\right)$,
the resisting force
$F_{\textsf{r}} = y^{\prime}$
(where $y^{\prime}$ is the first order time derivative of $y$),
and
the spring force
$F_{\textsf{s}} = k y$
(where $k = 4$ lb/ft is the spring constant).
Since we are setting the equilibrium point
at when the mass-spring system hangs freely,
and not when the spring alone hangs freely,
the effect of $F_{\textsf{m}}$
on the motion of the mass
can be sufficiently subscribed to $F_{\textsf{s}}$
(that is, we can neglect $F_{\textsf{m}}$).
By Newtonian steady-state mechanics,
the net effect of $F_{\textsf{d}}$, $F_{\textsf{r}}$, and $F_{\textsf{s}}$
corresponds to a proportional acceleration in the point mass:

$$
F_{\textsf{d}} - F_{\textsf{r}} - F_{\textsf{s}}
= m y^{\prime \prime}
\quad \Longrightarrow \quad
0.25 \sin \left(8t\right) - y^{\prime} - k y
= m y^{\prime \prime};
\quad k = 4,\ m = \frac{2}{32.17}
$$ (4.0a)
In other words,
we now have a second-order non-homogeneous linear ODE
as an initial value problem:

$$
y^{\prime \prime} + \frac{1}{m} y^{\prime} + \frac{k}{m} y
= \frac{1}{4m} \sin \left(8t\right);
\quad y \left(0\right) = -3,\ y^{\prime}\left(0\right) = 3
$$ (4.0b)

Ignoring the right-hand side of (4.0b),
we arrive at a homogeneous ODE whose characteristic equation is
$\lambda^{2} + \frac{1}{m} \lambda + \frac{k}{m} = 0$.
By the quadratic formula, the characteristic roots are

$$
\lambda_{1} = \frac{-1 + \sqrt{1 - 4km}}{2m},
\quad
\lambda_{2} = \frac{-1 - \sqrt{1 - 4km}}{2m}
$$ (4.1a)
Notice that, from (4.0a), $4km < 1$;
ergo, $\lambda_{1}$ and $\lambda_{2}$ are real and distinct.
The homogeneous solution is the superposition of
the basis functions
$\exp \left(\lambda_{1} t\right)$
and
$\exp \left(\lambda_{2} t\right)$:

$$
y_{\textsf{h}}
=
C_{1} \exp \left(\lambda_{1} t\right)
+
C_{2} \exp \left(\lambda_{2} t\right)
$$ (4.1b)
where $C_{1}$ and $C_{2}$ are constants.

Now, inspecting the right-hand side of (4.0b),
we can deduce that the particular solution
is a superposition of the basis functions
$\cos \left(8t\right)$
and
$\sin \left(8t\right)$:

$$
y_{\textsf{p}}
=
C_{3} \cos \left(8t\right)
+
C_{4} \sin \left(8t\right)
$$ (4.2a)
where $C_{3}$ and $C_{4}$ are constants.
The velocity and acceleration
based on $y_{\textsf{p}}$ would be

$$
y_{\textsf{p}}^{\prime}
=
8 C_{4} \cos \left(8t\right)
-
8 C_{3} \sin \left(8t\right),
\quad
y_{\textsf{p}}^{\prime \prime}
=
-64 C_{3} \cos \left(8t\right)
-
64 C_{4} \sin \left(8t\right)
$$
Substituting
$y_{\textsf{p}}$,
$y_{\textsf{p}}^{\prime}$,
and
$y_{\textsf{p}}^{\prime \prime}$
onto (4.0b),

$$
\left(
-64 C_{3} + \frac{k C_{3}}{m} + \frac{8 C_{4}}{m}
\right)
\cos \left(8t\right)
+
\left(
- \frac{8 C_{3}}{m} -64 C_{4} + \frac{k C_{4}}{m}
\right)
\sin \left(8t\right)
=
\frac{1}{4m}
\sin \left(8t\right)
$$
which gives

$$
C_{3} =
\frac{-8}{
256 + 4096 m^{2} - 128 mk + k^{2}
};
\quad
C_{4} =
\frac{-64m + k}{
256 + 4096 m^{2} - 128 mk + k^{2}
}
$$ (4.2b).

The complete solution to (4.0b)
is the superposition of
$y_{\textsf{h}}$ and $y_{\textsf{p}}$:

$$
y \left(t\right) =
C_{1} \exp \left(\lambda_{1} t\right)
+
C_{2} \exp \left(\lambda_{2} t\right)
+
C_{3} \cos \left(8t\right) + C_{4} \sin \left(8t\right)
$$ (4.3a)
where
$C_{1}$ and $C_{2}$ are yet unknown constants,
and

$$
\lambda_{1} = \frac{-1 + \sqrt{1 - 4km}}{2m},
\quad
\lambda_{2} = \frac{-1 - \sqrt{1 - 4km}}{2m}
$$ (4.3b)
$$
C_{3} =
\frac{-8}{
256 + 4096 m^{2} - 128 mk + k^{2}
};
\quad
C_{4} =
\frac{-64m + k}{
256 + 4096 m^{2} - 128 mk + k^{2}
}
$$ (4.3c)

The complete solution should meet the initial conditions.
Hence, for the initial position of the point mass,

$$
y \left(0\right)
=
C_{1} + C_{2} + C_{3}
=
-3
\quad \Longrightarrow \quad
C_{1} + C_{2} = - C_{3} - 3
$$ (4.4a)
For the initial velocity of the point mass,

$$
y^{\prime} \left(0\right)
=
\lambda_{1} C_{1} + \lambda_{2} C_{2} + 8 C_{4}
=
3
\quad \Longrightarrow \quad
\lambda_{1} C_{1} + \lambda_{2} C_{2} = -8 C_{4} + 3
$$ (4.4b)
Solving (4.4a) and (4.4b) for the unknowns,

$$
C_{1} =
\frac{\lambda_{2}}{\lambda_{1} - \lambda_{2}} C_{3}
-
\frac{8}{\lambda_{1} - \lambda_{2}} C_{4}
+
\frac{3 \left(1 + \lambda_{2}\right)}{\lambda_{1} - \lambda_{2}}
$$
$$
C_{2} =
\frac{- \lambda_{1}}{\lambda_{1} - \lambda_{2}} C_{3}
+
\frac{8}{\lambda_{1} - \lambda_{2}} C_{4}
-
\frac{3 \left(1 + \lambda_{1}\right)}{\lambda_{1} - \lambda_{2}}
$$
As expected,
$\lambda_{1}$, $\lambda_{2}$,
$C_{1}$, $C_{2}$, $C_{3}$, and $C_{4}$,
are all dependent on system parameters $k$ and $m$.

Therefore, the complete solution to
(4.0b)&ndash;*i.e.*,
the equation of motion for the point mass&ndash;expressed
in terms of $k$ and $m$, is

$$
y \left(t\right) =
C_{1} \exp \left(\lambda_{1} t\right)
+
C_{2} \exp \left(\lambda_{2} t\right)
+
C_{3} \cos \left(8t\right) + C_{4} \sin \left(8t\right)
$$ (4.5a)
$$
\lambda_{1} = \frac{-1 + \sqrt{1 - 4km}}{2m},
\quad
\lambda_{2} = \frac{-1 - \sqrt{1 - 4km}}{2m}
$$ (4.5b)
$$
C_{3} =
\frac{-8}{
256 + 4096 m^{2} - 128 mk + k^{2}
};
\quad
C_{4} =
\frac{-64m + k}{
256 + 4096 m^{2} - 128 mk + k^{2}
}
$$ (4.5c)
$$
C_{1} =
\frac{\lambda_{2}}{\lambda_{1} - \lambda_{2}} C_{3}
-
\frac{8}{\lambda_{1} - \lambda_{2}} C_{4}
+
\frac{3 \left(1 + \lambda_{2}\right)}{\lambda_{1} - \lambda_{2}};
\quad
C_{2} =
\frac{- \lambda_{1}}{\lambda_{1} - \lambda_{2}} C_{3}
+
\frac{8}{\lambda_{1} - \lambda_{2}} C_{4}
-
\frac{3 \left(1 + \lambda_{1}\right)}{\lambda_{1} - \lambda_{2}}
$$ (4.5d)
Substituting $k = 4$, $m = \frac{2}{g}$, and $g = 32.17$,
and rounding up floating-point terms to three decimal places,

$$
y \left(t\right) =
-19.339 \exp \left(-7.458 t\right)
+
16.370 \exp \left(-8.627 t\right)
-
0.031 \cos \left(8t\right)
+
8.257 \times 10^{-5} \sin \left(8t\right)
$$ (4.5e)

# Problem V

A coil of inductance 1 henry
and negligible resistance
is connected in series with
a capacitance of $10^{-6}$ farads
and
an EMF of $E$ volts.
Taking $Q = I = 0$ at time $t = 0$,
find the charge $Q$
and the current $I$
when $t = 0.001$ s
if
(a) $E = 100$ volts;
(b) $E = 100 \sin 500t$ volts;
and
(c) $E = 100 \sin 1000t$ volts.

Here we see a three-element circuit.
From elementary electromagnetics,
the current can be described as
a time rate of change of charge:

$$
I \left(t\right) = \frac{d Q \left(t\right)}{dt}
$$ (5.0a)
The voltage drop across a coil due to self-inductance is
proportional to the rate of change of the current through that coil.
In the present problem where the current through the coil
is the same all throughout the circuit,

$$
v_{\textsf{L}} \left(t\right) = L \frac{d I \left(t\right)}{dt}
$$ (5.0b)
where $L = 1$ H is the inductance.
Since an inductor does not store energy in the form of charges,
and resistive elements are neglected in the problem,
then the charge stored in the capacitor
is also that which "flows" in the entirety of the circuit.
The voltage drop across the capacitor,
being proportional to the charge stored,
is

$$
v_{\textsf{C}} \left(t\right) = \frac{1}{C} Q \left(t\right)
$$ (5.0c)
where $C = 10^{-6}$ F is the capacitance.
By Kirchhoff, the algebraic sum of the voltage drops
across the elements of the circuit at any instant
must be equal to zero:

$$
E \left(t\right)
=
v_{\textsf{L}} \left(t\right) + v_{\textsf{C}} \left(t\right)
=
L \frac{d I \left(t\right)}{dt} + \frac{1}{C} Q \left(t\right)
$$ (5.0d)
From (5.0a), we can rewrite (5.0d) as an
initial value problem based on a
second-order non-homogeneous linear ODE:

$$
Q^{\prime \prime} + \frac{1}{LC} Q = \frac{E}{L}
;\quad
Q \left(0\right) = 0,\ 
Q^{\prime} \left(0\right) = 0
;\quad
L = 1,\ C = 10^{-6}
$$ (5.0e)
where
$Q^{\prime} = I$
and the explicit indications of time-dependence
are dropped for brevity.

## (a) $E = 100$ V

With $E = 100$ V,

$$
Q^{\prime \prime} + \frac{1}{LC} Q = \frac{100}{L}
;\quad
Q \left(0\right) = 0,\ 
Q^{\prime} \left(0\right) = 0
;\quad
L = 1,\ C = 10^{-6}
$$ (5.1)

Neglecting the right-hand side of (5.1),
we get a homogeneous ODE whose characteristic equation is
$\lambda^{2} + \frac{1}{LC} = 0$.
This leads to two real and distinct characteristic roots:
$\lambda_{1} = \frac{1}{\sqrt{LC}}$
and
$\lambda_{2} = - \frac{1}{\sqrt{LC}}$.
The homogeneous solution would then be a superposition of basis functions
$\exp \left(\lambda_{1} t\right)$
and
$\exp \left(\lambda_{2} t\right)$:

$$
Q_{\textsf{h}}
=
C_{1} \exp \left(\frac{t}{\sqrt{LC}}\right)
+
C_{2} \exp \left(\frac{-t}{\sqrt{LC}}\right)
$$ (5.2)
where $C_{1}$ and $C_{2}$ are constants.
Moreover, we can deduce from the right-hand side of (5.1)
that the particular solution is of the form
$Q_{\textsf{p}} = C_{3}$,
where $C_{3}$ is a constant.
Invoking $Q_{\textsf{p}}$ on (5.1),

$$
\frac{1}{LC} C_{3} = \frac{100}{L}
\quad \Longrightarrow \quad
C_{3} = 100 C
$$
Hence, the particular solution is

$$
Q_{\textsf{p}} = 100 C
$$ (5.3)
The complete solution is then the superposition of
$Q_{\textsf{h}}$ and $Q_{\textsf{p}}$:

$$
Q = Q_{\textsf{h}} + Q_{\textsf{p}}
=
C_{1} \exp \left(\frac{t}{\sqrt{LC}}\right)
+
C_{2} \exp \left(\frac{-t}{\sqrt{LC}}\right)
+ 100C
;\quad
L = 1,\ C = 10^{-6}
$$ (5.4)
where $C_{1}$ and $C_{2}$ are constants.
The initial conditions state that the circuit was devoid of charges:

$$
Q \left(0\right) = C_{1} + C_{2} + 100 C = 0
\quad \Longrightarrow \quad
C_{1} + C_{2} = - 100C

$$
and
had no current flow:

$$
Q^{\prime} \left(0\right)
=
\lambda_{1} C_{1} + \lambda_{2} C_{2} = 0
\quad \Longrightarrow \quad
\lambda_{1} C_{1} + \lambda_{2} C_{2} = 0
$$
whence
$C_1 = C_2 = - 50C$.
Therefore, the complete solution to (5.1)&ndash;*i.e.*,
the instantaneous charge&ndash;is

$$
Q =
-50C \exp \left(\frac{t}{\sqrt{LC}}\right)
-50C \exp \left(\frac{-t}{\sqrt{LC}}\right)
+ 100C
;\quad
L = 1,\ C = 10^{-6}
$$ (5.5a)
The instantaneous current is then

$$
I =
-50 \sqrt{\frac{C}{L}} \exp \left(\frac{t}{\sqrt{LC}}\right)
+ 50C \sqrt{\frac{C}{L}} \exp \left(\frac{-t}{\sqrt{LC}}\right)
;\quad
L = 1,\ C = 10^{-6}
$$ (5.5b)

At $t=0.001$,

$$
Q \left(0.001\right)
\approx
- 5.43081 \times 10^{-5}
\text{ coulumbs}
;\quad
I \left(0.001\right)
\approx
- 0.11752
\text{ amperes}
$$

## (b) $E = 100 \sin \left(500t\right)$ V

With $E = 100 \sin \left(500t\right)$ V,

$$
Q^{\prime \prime} + \frac{1}{LC} Q = \frac{100}{L} \sin \left(500t\right)
;\quad
Q \left(0\right) = 0,\ 
Q^{\prime} \left(0\right) = 0
;\quad
L = 1,\ C = 10^{-6}
$$ (5.6)

Since the only difference between (5.1) and (5.6)
is in their right-hand sides,
the homogeneous solution to (5.6)
is that given in (5.2):

$$
Q_{\textsf{h}}
=
C_{1} \exp \left(\frac{t}{\sqrt{LC}}\right)
+
C_{2} \exp \left(\frac{-t}{\sqrt{LC}}\right)
$$ (5.2)
where $C_{1}$ and $C_{2}$ are constants.
Now looking at the right-hand side of (5.6),
we can deduce that the particular solution is of the form

$$
Q_{\textsf{p}}
=
C_{3} \cos \left(500t\right)
+
C_{4} \sin \left(500t\right)
$$
where $C_{3}$ and $C_{4}$ are constants.
Applying $Q_{\textsf{p}}$ onto (5.6),

$$
\left(
    - 2.5 \times 10^5
    + \frac{1}{LC}
\right)
C_3 \cos \left(500t\right)
+
\left(
    - 2.5 \times 10^5
    + \frac{1}{LC}
\right)
C_4 \sin \left(500t\right)
=
\frac{100}{L} \sin \left(500t\right)
$$
which gives

$$
C_{3} = 0
;\quad
C_{4} =
\frac{100C}{1 - 2.5\times10^{5} LC}
$$
Hence, the particular solution is

$$
Q_{\textsf{p}}
=
\frac{100C}{1 - 2.5\times10^{5} LC}
\sin \left(500t\right)
$$ (5.7)
The complete solution is then the superposition of
$Q_{\textsf{h}}$ and $Q_{\textsf{p}}$:

$$
Q = Q_{\textsf{h}} + Q_{\textsf{p}}
=
C_{1} \exp \left(\frac{t}{\sqrt{LC}}\right)
+
C_{2} \exp \left(\frac{-t}{\sqrt{LC}}\right)
+
C_{4} \sin \left(500t\right)
;\quad
C_{4} =
\frac{100C}{1 - 2.5\times10^{5} LC}
$$ (5.8)
where
$L = 1$, $C = 10^{-6}$,
and $C_{1}$ and $C_{2}$ are yet unknown constants.
The initial conditions state that the circuit was devoid of charges:

$$
Q \left(0\right) = C_{1} + C_{2} = 0
\quad \Longrightarrow \quad
C_{1} + C_{2} = 0

$$
and
had no current flow:

$$
Q^{\prime} \left(0\right)
=
\lambda_{1} C_{1} + \lambda_{2} C_{2}
+
500 C_{4}
= 0
\quad \Longrightarrow \quad
\lambda_{1} C_{1} + \lambda_{2} C_{2} =
-500 C_{4}
$$
where $\lambda_{1}$ and $\lambda_{2}$
are as defined in (5.2).
This gives
$C_{1} = -250 \sqrt{LC} C_{4}$
and
$C_{2} = 250 \sqrt{LC} C_{4}$.
Therefore,
the instantaneous charge
and
the instantaneous current
are

$$
Q =
C_{1} \exp \left(\frac{t}{\sqrt{LC}}\right)
+
C_{2} \exp \left(\frac{-t}{\sqrt{LC}}\right)
+
C_{4} \sin \left(500t\right)
$$ (5.9a)
$$
I =
\frac{C_{1}}{\sqrt{LC}} \exp \left(\frac{t}{\sqrt{LC}}\right)
-
\frac{C_{2}}{\sqrt{LC}} \exp \left(\frac{-t}{\sqrt{LC}}\right)
+
500 C_{4} \cos \left(500t\right)
$$ (5.9b)
where $L = 1$, $C = 10^{-6}$,
and

$$
C_{4} =
\frac{100C}{1 - 2.5\times10^{5} LC}
;\quad
C_{1} = -250 \sqrt{LC} C_{4}
;\quad
C_{2} = 250 \sqrt{LC} C_{4}
$$ (5.9c)

At $t=0.001$,

$$
Q \left(0.001\right)
\approx
-1.44233 \times 10^{-5}
\text{ coulumbs}
;\quad
I \left(0.001\right)
\approx
-0.04437
\text{ amperes}
$$

## (c) $E = 100 \sin \left(1000t\right)$ V

With $E = 100 \sin \left(1000t\right)$ V,

$$
Q^{\prime \prime} + \frac{1}{LC} Q = \frac{100}{L} \sin \left(1000t\right)
;\quad
Q \left(0\right) = 0,\ 
Q^{\prime} \left(0\right) = 0
;\quad
L = 1,\ C = 10^{-6}
$$ (5.10)

Since the only difference between (5.1) and (5.10)
is in their right-hand sides,
the homogeneous solution to (5.10)
is that given in (5.2):

$$
Q_{\textsf{h}}
=
C_{1} \exp \left(\frac{t}{\sqrt{LC}}\right)
+
C_{2} \exp \left(\frac{-t}{\sqrt{LC}}\right)
$$ (5.2)
where $C_{1}$ and $C_{2}$ are constants.
Now looking at the right-hand side of (5.10),
we can deduce that the particular solution is of the form

$$
Q_{\textsf{p}}
=
C_{3} \cos \left(1000t\right)
+
C_{4} \sin \left(1000t\right)
$$
where $C_{3}$ and $C_{4}$ are constants.
Applying $Q_{\textsf{p}}$ onto (5.10),

$$
\left(
    - 1 \times 10^6
    + \frac{1}{LC}
\right)
C_3 \cos \left(1000t\right)
+
\left(
    - 1 \times 10^6
    + \frac{1}{LC}
\right)
C_4 \sin \left(1000t\right)
=
\frac{100}{L} \sin \left(1000t\right)
$$
which gives

$$
C_{3} = 0
;\quad
C_{4} =
\frac{100C}{1 - 1\times10^{6} LC}
$$
Hence, the particular solution is

$$
Q_{\textsf{p}}
=
\frac{100C}{1 - 1\times10^{6} LC}
\sin \left(1000t\right)
$$ (5.11)
The complete solution is then the superposition of
$Q_{\textsf{h}}$ and $Q_{\textsf{p}}$:

$$
Q = Q_{\textsf{h}} + Q_{\textsf{p}}
=
C_{1} \exp \left(\frac{t}{\sqrt{LC}}\right)
+
C_{2} \exp \left(\frac{-t}{\sqrt{LC}}\right)
+
C_{4} \sin \left(1000t\right)
;\quad
C_{4} =
\frac{100C}{1 - 1\times10^{6} LC}
$$ (5.12)
where
$L = 1$, $C = 10^{-6}$,
and $C_{1}$ and $C_{2}$ are yet unknown constants.
The initial conditions state that the circuit was devoid of charges:

$$
Q \left(0\right) = C_{1} + C_{2} = 0
\quad \Longrightarrow \quad
C_{1} + C_{2} = 0

$$
and
had no current flow:

$$
Q^{\prime} \left(0\right)
=
\lambda_{1} C_{1} + \lambda_{2} C_{2}
+
1000 C_{4}
= 0
\quad \Longrightarrow \quad
\lambda_{1} C_{1} + \lambda_{2} C_{2} =
-1000 C_{4}
$$
where $\lambda_{1}$ and $\lambda_{2}$
are as defined in (5.2).
This gives
$C_{1} = -500 \sqrt{LC} C_{4}$
and
$C_{2} = 500 \sqrt{LC} C_{4}$.
Therefore,
the instantaneous charge
and
the instantaneous current
are

$$
Q =
C_{1} \exp \left(\frac{t}{\sqrt{LC}}\right)
+
C_{2} \exp \left(\frac{-t}{\sqrt{LC}}\right)
+
C_{4} \sin \left(1000t\right)
$$ (5.13a)
$$
I =
\frac{C_{1}}{\sqrt{LC}} \exp \left(\frac{t}{\sqrt{LC}}\right)
-
\frac{C_{2}}{\sqrt{LC}} \exp \left(\frac{-t}{\sqrt{LC}}\right)
+
1000 C_{4} \cos \left(1000t\right)
$$ (5.13b)
where $L = 1$, $C = 10^{-6}$,
and

$$
C_{4} =
\frac{100C}{1 - 1\times10^{6} LC}
;\quad
C_{1} = -500 \sqrt{LC} C_{4}
;\quad
C_{2} = 500 \sqrt{LC} C_{4}
$$ (5.13c)

Notice that,
when plugging in
$L = 1$ and $C = 10^{-6}$,
the coefficient $C_4$ tends to infinity.
This means that at $t > 0$,
such as $t=0.001$,
the charge and the current have grown out of bounds:

$$
Q \left(0.001\right)
\rightarrow
\infty
\text{ coulumbs}
;\quad
I \left(0.001\right)
\rightarrow
\infty
\text{ amperes}
$$
This occurs because the driving source
oscillates at a frequency ($1000$) that matches
the natural frequency ($\frac{1}{\sqrt{LC}}$) of the circuit.