# Answers to Problem Set II <!-- omit in toc -->

*Prepared by*
Christian Y. Cahig

# Problem 1

Solve the following ODE:
$$
\left(x^2y + y^3 - y\right) dx
+
\left(x^3 + xy^2 + x\right) dy
=
0
$$ (1.0)

Factoring and dividing both sides of (1.0) by
$x^2 + y^2$,
$$
\frac{
    \left[\left(x^2 + y^2\right) y - y\right]
}{x^2 + y^2}
dx
+
\frac{
    \left[\left(x^2 + y^2\right) x + x\right]
}{x^2 + y^2}
dy
=
0
$$
which simplifies to
$$
ydx + xdy
+
\frac{xdy - ydx}{x^2 + y^2}
=
0
$$ (1.1)

Observe that
the full differential of
$xy$ 
is given by
$$
d \left(xy\right)
=
\frac{\partial}{\partial x}
\left(xy\right)
dx
+
\frac{\partial}{\partial y}
\left(xy\right)
dy
=
ydx + xdy
$$ (1.2)
In the same manner,
the full differential of
$\arctan \frac{y}{x}$
is given by
$$
d \left(\arctan \frac{y}{x}\right)
=
\frac{\partial}{\partial x}
\left(\arctan \frac{y}{x}\right)
dx
+
\frac{\partial}{\partial y}
\left(\arctan \frac{y}{x}\right)
dy
=
\frac{- ydx + xdy}{x^2 + y^2}
$$ (1.3)
In other words,
the given ODE is equivalent to
$$
d \left(xy\right)
+
d \left(\arctan \frac{y}{x}\right)
=
0
$$ (1.4)

Integrating both sides of (1.4),
$$
\int d \left(xy\right)
+
\int d \left(\arctan \frac{y}{x}\right)
=
\int 0
\quad \Longrightarrow \quad
xy + \arctan \frac{y}{x} + C = 0
$$
where
$C$ collectively denotes the constants of integration.
With some abuse of notation,
the solution to (1.0) is
$$
xy + \arctan \frac{y}{x} = C
$$ (1.5)
where $C$ is a constant.

# Problem 2

Solve the following ODE:
$$
y dx + x dy + y^2 dy = 0
$$ (2.0)

Basic algebraic manipulation of (2.0) yields
$$
y dx
+
\left(x + y^2\right) dy
=
0
$$ (2.1)
Assume that (2.1) describes the
full differential of a function
$u \left(x,y\right) = C$,
where $C$ is some constant.
As such,
we can say that
$$
u \left(x,y\right) = C
\quad \Longrightarrow \quad
\frac{\partial u}{\partial x} dx
+
\frac{\partial u}{\partial y} dy
=
0
$$
which, when compared to (2.1), yields
$$
\frac{\partial u}{\partial x} = y
$$ (2.2a)
$$
\frac{\partial u}{\partial y} = x + y^2
$$ (2.2b)

Differentiating (2.2a) with respect to $y$
and (2.2b) with respect to $x$
will show that (2.0) is an exact ODE:
$$
\frac{\partial}{\partial y}
\left(\frac{\partial u}{\partial x}\right)
= 1 =
\frac{\partial}{\partial x}
\left(\frac{\partial u}{\partial y}\right)
$$
This means that $u \left(x,y\right)$ is given by
$$
u \left(x,y\right)
=
\int \frac{\partial u}{\partial x} dx
+
K \left(y\right)
$$ (2.3)
where $K \left(y\right)$
is some function of $y$.
Substituting (2.2a) onto (2.3),
$$
u \left(x,y\right)
=
\int y dx
+
K \left(y\right)
=
xy + K \left(y\right)
$$ (2.4)
Differentiating both sides of (2.4)
with respect to $y$
and invoking (2.2b),
$$
\frac{\partial u \left(x,y\right)}{\partial y}
=
x
+
\frac{\partial K \left(y\right)}{\partial y}
=
x + y^2
$$
whence
$$
\frac{\partial K \left(y\right)}{\partial y}
=
\frac{dK}{dy}
=
y^2
$$ (2.5)
Notice that (2.5) is a separable ODE,
*i.e.*
$$
dK = y^2 dy
\quad \Longrightarrow \quad
\int dK = \int y^2 dy
\quad \Longrightarrow \quad
K \left(y\right)
=
\frac{1}{3} y^3 + \tilde{C}
$$ (2.6)
where $\tilde{C}$
is a constant of integration.
Substituting (2.6) onto (2.4),
$$
xy + \frac{1}{3} y^3 + \tilde{C} = C
$$
With some simplification
and an abuse of notation,
the solution to (2.0) is
$$
3xy + y^3 = C
$$ (2.7)

# Problem 3

Solve the following ODE:
$$
t ds
=
\left(3t + 1\right) s dt
+
t^3 e^{3t} dt
$$ (3.0)

We can rewrite (3.0) as
$$
t ds
-
\left[
\left(3t + 1\right) s
+
t^3 e^{3t}
\right]
dt
=
0
$$ (3.1)
It is trivial
that differentiating
$t$ with respect to $t$
yields an expression
different to differentiating
$-
\left[
\left(3t + 1\right) s
+
t^3 e^{3t}
\right]$
with respect to $s$.
In other words,
(3.0) is an inexact ODE.

For convenience,
we denote the factors of
$ds$ and of $dt$ as
$M$ and $N$,
respectively.
We then define a quantity $R \left(t\right)$ as
$$
R\left(t\right) =
\frac{1}{M}
\left(
\frac{dN}{ds} - \frac{dM}{dt}
\right)
=
\frac{1}{t}
\left(
- 3t - 1 - 1
\right)
=
-3 - 2t^{-1}
$$ (3.2)
Seeing that $R \left(t\right)$
is a function of $t$ alone,
we can define a suitable integrating factor
$F \left(t\right)$
as
$$
F \left(t\right)
=
\exp \left[\int R \left(t\right) dt\right]
=
\exp \left[\int \left(-3 - 2t^{-1}\right) dt\right]
=
\exp \left(-3t\right)
\exp \left(-2 \ln |t| \right)
=
t^{-2} e^{-3t}
$$ (3.3)

Multiplying both sides of (3.1) by $F \left(t\right)$ yields
$$
t^{-1} e^{-3t}
ds
-
\left[
\left(3t^{-1} e^{-3t} + t^{-2} e^{-3t}\right) s
+
t
\right]
dt
=
0
$$ (3.4)
Let $P$ and $Q$
be the respective factors
of $ds$ and of $dt$
in (3.4).
Differentiating
$P$ with respect to $t$
and
$Q$ with respect to $s$
confirms that (3.4) is now an exact ODE:
$$
\frac{dP}{dt}
=
\frac{dQ}{ds}
\quad \colon \quad
\frac{\partial}{\partial t}
\left(t^{-1} e^{-3t}\right)
=
-3 t^{-1} e^{-3t} - t^{-2} e^{-3t}
=
\frac{\partial}{\partial s}
\left[
- \left(3t^{-1} e^{-3t} + t^{-2} e^{-3t}\right) s
- t
\right]
$$
As such,
we can assume that
the solution to
(3.4)&ndash;and hence, to (3.0)&ndash;is
the multivariate function
$u \left(s,t\right) = C$,
where $C$ is some constant.
The full differential of
$u \left(s,t\right)$
is (3.4),
*i.e.*,
$$
\frac{\partial u}{\partial s}
= P
=
t^{-1} e^{-3t}
\quad , \quad
\frac{\partial u}{\partial t}
= Q
=
- \left(3t^{-1} e^{-3t} + t^{-2} e^{-3t}\right) s
- t
$$
Moreover,
$u \left(s,t\right)$
can be expressed as
$$
u \left(s,t\right)
=
\int \frac{\partial u}{\partial s} ds
+
K \left(t\right)
=
\int P ds + K \left(t\right)
$$
where $K \left(t\right)$ is a function of $t$.
Evaluating,
$$
u \left(s,t\right)
=
\int t^{-1} e^{-3t} ds
+
K \left(t\right)
=
s t^{-1} e^{-3t} + K \left(t\right)
$$ (3.5)
Differentiating both sides of (3.5)
with respect to $t$,
and invoking $Q$,
$$
\frac{\partial u \left(s,t\right)}{\partial t}
=
Q
\quad \colon \quad
-
\left(3 t^{-1} e^{-3t} + t^{-2} e^{-3t}\right)
s
+
\frac{\partial K \left(t\right)}{\partial t}
=
-
\left(3 t^{-1} e^{-3t} + t^{-2} e^{-3t}\right)
s
- t 
$$
Hence,
$$
\frac{\partial K \left(t\right)}{\partial t}
=
\frac{dK}{dt}
=
- t
$$ (3.6)

Since (3.6) is a separable ODE,
$$
dK = -t dt
\quad \Longrightarrow \quad
\int dK = \int -t dt
\quad \Longrightarrow \quad
K \left(t\right) = -
\frac{1}{2}
t^{2}
+ \tilde{C}
$$ (3.7)
where $\tilde{C}$ is a constant of integration.
Substituting (3.7) onto (3.5),
$$
u \left(s,t\right)
=
s t^{-1} e^{-3t}
-
\frac{1}{2}
t^{2}
+ \tilde{C}
= C
$$
Simplifying and subscribing all constants to $C$,
the solution to (3.0) is
$$
2 s t^{-1} e^{-3t}
- t^{2} = C
$$ (3.8)

# Problem 4

Solve the following ODE:
$$
2 x^3 y^{\prime}
= y \left(y^2 + 3 x^2\right)
$$ (4.0)

By algebraic manipulation,
we can rewrite (4.0) as
$$
y^{\prime}
-
\frac{3}{2x}
y
=
\frac{1}{2x^3}
y^3
$$ (4.1)
where $y$ is understood to be a function of $x$.
By Kreyzsig's convention,
(4.1) is a Bernoulli ODE with
$$
P \left(x\right)
=
- \frac{3}{2x}
\quad , \quad
G \left(x\right)
=
\frac{1}{2 x^3}
\quad , \quad
\alpha = 3
$$ (4.2)

Employing an auxiliary variable change,
$$
u = y^{1 - \alpha} = y^{-2}
\quad \Longrightarrow \quad
u^{\prime} = -2 y^{-3} y^{\prime}
$$ (4.3)
and substituting onto (4.1)
will give a reduced linear ODE:
$$
u^{\prime}
+
(1 - \alpha)
P \left(x\right)
u
=
(1 - \alpha)
G \left(x\right)
\quad \Longrightarrow \quad
u^{\prime} + 3 x^{-1} u = - x^{-3}
$$ (4.4)

The solution to (4.4)
is readily given as
$$
u
=
e^{-H \left(x\right)}
\left[
\int e^{H \left(x\right)}
\left(-x^{-3}\right)
dx
+
C
\right]
$$ (4.5)
where $C$ is a constant
and
$$
H \left(x\right)
=
\int 3 x^{-1} dx
=
3 \ln |x|
$$
Evaluating (4.5),
$$
e^{- H \left(x\right)}
= e^{-3 \ln |x|}
= e^{-3 \ln x}
= x^{-3}
$$
$$
e^{H \left(x\right)}
= e^{3 \ln |x|}
= e^{3 \ln x}
= x^{3}
$$
$$
u
= x^{-3}
\int (x^{3})(-x^{-3}) dx
+ C x^{-3}
= - x^{-2} + C x^{-3}
$$ (4.6)

Substituting back (4.3) onto (4.6),
$$
y^{-2}
= - x^{-2} + C x^{-3}
$$
Isolating $C$ on one side,
the solution to (4.0)
can be written as
$$
\frac{x^3 + xy^2}{y^2}
= C
$$ (4.7)

# Problem 5

Solve the following ODE:
$$
2 wt \frac{dt}{dw} = t^2 - 2 w^3
$$ (5.0)

For brevity,
let $t^{\prime}$
denote the derivative of $t$
with respect to $w$,
implying of course that
$t$ is a function of $w$.
Applying this
and algebraic manipulation
to (5.0),
we get an equivalent
expression of the given ODE:
$$
t^{\prime}
- \frac{1}{2w} t
= - w^2 t^{-1}
$$ (5.1)
By Kreyzsig's convention,
(5.1) is a Bernoulli ODE with
$$
P \left(w\right)
=
- \frac{1}{2w}
\quad , \quad
G \left(w\right)
=
- w^2
\quad , \quad
\alpha = -1
$$ (5.2)

Employing an auxiliary variable change,
$$
y = t^{1 - \alpha} = t^{2}
$$ (5.3)
and substituting onto (5.1)
will give a reduced linear ODE:
$$
y^{\prime}
- \frac{1}{w} y
= - 2 w^2
$$ (5.4)

The solution to (5.4)
is readily given as
$$
y
=
e^{-H \left(w\right)}
\left[
\int e^{H \left(w\right)}
\left(-2 w^2\right)
dw
+
C
\right]
$$ (5.5)
where $C$ is a constant
and
$$
H \left(w\right)
=
\int - \frac{1}{w} dw
=
- \ln |w|
$$
Evaluating (5.5),
$$
e^{- H \left(w\right)}
= e^{\ln |w|}
= e^{\ln w}
= w
; \quad w > 0
$$
$$
e^{H \left(w\right)}
= e^{- \ln |w|}
= e^{- \ln w}
= w^{-1}
; \quad w > 0
$$
$$
y
= w
\int (w^{-1})(-2 w^2) dw
+ Cw
= - w^3 + Cw
$$ (5.6)

Substituting back (5.3) onto (5.6),
$$
t^2 = - w^{-3} + Cw
$$
Isolating $C$ on one side,
the solution to (5.0)
can be written as
$$
\frac{t^2 + w^3}{w}
= C
$$ (5.7)