# Answers to Problem Set V

*Prepared by*
Christian Y. Cahig

## Problem I

Find the power series solution (in $x$) of the following ODE:

$$
y^{\prime \prime} + 2 x y^{\prime} + y = 0
$$ (1.0)

We assume that the solution $y$ is a power series solution:

$$
y = \sum_{m=0}^{\infty} a_{m} x^{m}
$$ (1.1)
where the $a_{n}$ terms are constant coefficients.
Differentiating $y$ with respect to $x$,

$$
y^{\prime} = \sum_{m=1}^{\infty} m a_{m} x^{m-1}
\\
y^{\prime \prime} = \sum_{m=2}^{\infty} m \left(m - 1\right) a_{m} x^{m-2}
$$ (1.2)
Substituting (1.2) onto (1.0),

$$
\sum_{m=2}^{\infty} m \left(m - 1\right) a_{m} x^{m-2}
+
2 \sum_{m=1}^{\infty} m a_{m} x^{m}
+
\sum_{m=0}^{\infty} a_{m} x^{m}
= 0
$$
The first series can be re-written
in terms of $x^{m}$, *i.e.*,

$$
\sum_{m=2}^{\infty} m \left(m - 1\right) a_{m} x^{m-2}
=
\sum_{m=0}^{\infty} \left(m + 2\right) \left(m + 1\right) a_{m+2} x^{m}
$$
Moreover, notice that the index of second series in (1.3) can start at $m = 0$:

$$
\sum_{m=1}^{\infty} m a_{m} x^{m}
=
0 \cdot a_{0} x^{0} + 1 \cdot a_{1} x^{1} + 2 \cdot a_{2} x^{2} + \cdots
=
\sum_{m=0}^{\infty} m a_{m} x^{m}
$$
The series equivalent of the given ODE can now be expressed
in terms of $x^{m}$ and with indices starting at 0:

$$
\sum_{m=0}^{\infty}
\left[\left(m + 2\right) \left(m + 1\right) a_{m+2} + \left(2m + 1\right) a_{m}\right]
x^{m} =0
$$ (1.3)
The homogeneity of the given ODE means that the corresponding coefficient
of $x^{m}$ in (1.3) is zero, that is,

$$
a_{m+2} = -
\frac{2m + 1}{\left(m + 1\right) \left(m + 2\right)}
a_{m},
\quad m = 0,1,2,\ldots
$$ (1.4a)
Note that $a_{0}$ and $a_{1}$ cannot be determined from the recurrence relation alone,
and hence in the present treatment will be as arbitrary constants
derived from additional information (*e.g.*, initial conditions).
Moreover, the recurrence relation can be "split" into odd and even terms:

$$
a_{2k} = \left(-1\right)^{k} a_{0}
\prod_{j=0}^{k-1} \frac{4j + 1}{\left(2j + 1\right) \left(2j + 2\right)},
\quad k = 1,2,3,\ldots
$$ (1.4b)
$$
a_{2k+1} = \left(-1\right)^{k} a_{1}
\prod_{j=0}^{k-1} \frac{4j + 3}{\left(2j + 2\right) \left(2j + 3\right)},
\quad k = 1,2,3,\ldots
$$ (1.4c)
Therefore, we can write the series solution to (1.0) as

$$
y =
a_{0} \left[
    1 + \sum_{k=1}^{\infty} \left(-1\right)^{k}
    \prod_{j=0}^{k-1} \frac{4j + 1}{\left(2j + 1\right) \left(2j + 2\right)} x^{2k}
\right]
+
a_{1} \left[
    x + \sum_{k=1}^{\infty} \left(-1\right)^{k}
    \prod_{j=0}^{k-1} \frac{4j + 3}{\left(2j + 2\right) \left(2j + 3\right)} x^{2k+1}
\right]
$$ (1.5)
where $a_{0}$ and $a_{1}$ are constants.

## Problem II

Find the power series solution (in $x$) of the following ODE:

$$
y^{\prime \prime} - 4 x y^{\prime} + \left(4 x^{2} - 2\right) y = 0
$$ (2.0)

We assume that the solution $y$ is a power series solution:

$$
y = \sum_{m=0}^{\infty} a_{m} x^{m}
$$ (2.1)
where the $a_{n}$ terms are constant coefficients.
Differentiating $y$ with respect to $x$,

$$
y^{\prime} = \sum_{m=1}^{\infty} m a_{m} x^{m-1}
\\
y^{\prime \prime} = \sum_{m=2}^{\infty} m \left(m - 1\right) a_{m} x^{m-2}
$$ (2.2)
Substituting (2.2) onto (2.0),

$$
\sum_{m=2}^{\infty} m \left(m - 1\right) a_{m} x^{m-2}
- 4 \sum_{m=1}^{\infty} m a_{m} x^{m}
+ 4 \sum_{m=0}^{\infty} m a_{m} x^{m+2}
- 2 \sum_{m=0}^{\infty} m a_{m} x^{m}
= 0
$$ (2.1a)

Expressing all series terms (2.1a) in $x^{m}$,

$$
\sum_{m=0}^{\infty} \left(m + 2\right) \left(m + 1\right) a_{m+2} x^{m}
- 4 \sum_{m=0}^{\infty} m a_{m} x^{m}
+ 4 \sum_{m=2}^{\infty} a_{m-2} x^{m}
- 2 \sum_{m=0}^{\infty} a_{m} x^{m}
= 0
$$ (2.1b)
Note that

$$
\sum_{m=0}^{\infty} \left(m + 2\right) \left(m + 1\right) a_{m+2} x^{m}
= 2 a_{2} + 6 a_{3} x
+ \sum_{m=2}^{\infty} \left(m + 2\right) \left(m + 1\right) a_{m+2} x^{m}
$$

$$
\sum_{m=0}^{\infty} m a_{m} x^{m}
= a_{1} x + \sum_{m=2}^{\infty} m a_{m} x^{m}
$$

$$
\sum_{m=0}^{\infty} a_{m} x^{m}
= a_{0} + a_{1} x + \sum_{m=2}^{\infty} a_{m} x^{m}
$$
Hence, we can rewrite the series terms in (2.1b) to have indices starting at $m=2$:

$$
2a_{2} + 6a_{3}x - 6a_{1}x - 2a_{0}
+ \sum_{m=2}^{\infty}
\left[ \left(m+2\right)\left(m+1\right) a_{m+2} - \left(4m+2\right) a_{m} + 4 a_{m-2} \right]
x^{m} = 0
$$ (2.1c)

Since (2.0) is homogenous, it follows from (2.1c) that

$$
2a_{2} - 2a_{0} = 0 \Longrightarrow a_{2} = a_{0}
$$ (2.2a)
$$
6a_{3} - 6a_{1} = 0 \Longrightarrow a_{3} = a_{1}
$$ (2.2b)
$$
\left(m+2\right)\left(m+1\right) a_{m+2} - \left(4m+2\right) a_{m} + 4 a_{m-2} = 0
\Longrightarrow
a_{m+2} = \frac{\left(4m+2\right) a_{m} - 4 a_{m-2}}{\left(m+1\right)\left(m+2\right)}
$$ (2.2c)
Now, with $m=2,3,4,5,6,7,9$,

$$
a_{4} = \frac{a_{0}}{2},\ 
a_{6} = \frac{a_{0}}{6},\ 
a_{8} = \frac{a_{0}}{24};
\quad
a_{5} = \frac{a_{1}}{2},\ 
a_{7} = \frac{a_{1}}{6},\ 
a_{9} = \frac{a_{1}}{24}
$$
This suggests two patterns for when even and odd $m$'s:

$$
a_{0},\ a_{2} = a_{0},\ a_{4} = \frac{a_{0}}{2},\ a_{6} = \frac{a_{0}}{6},\ 
a_{8} = \frac{a_{0}}{24},\ 
\cdots\ \Longrightarrow\ 
a_{2k} = \frac{a_{0}}{k!},
\quad k=0,1,2,\ldots
\ \ \ \ \ \ \ 
$$

$$
a_{1},\ a_{3} = a_{1},\  a_{5} = \frac{a_{1}}{2},\  a_{7} = \frac{a_{1}}{6},\ 
a_{9} = \frac{a_{1}}{24},\ 
\cdots\ \Longrightarrow\ 
a_{2k+1} = \frac{a_{1}}{k!},
\quad k=0,1,2,\ldots
$$
Notice that any $a_{m}$ is dependent on either $a_{0}$ or $a_{1}$,
but $a_{0}$ and $a_{1}$ cannot be determined solely from the recurrence relations.
We can treat $a_{0}$ and $a_{1}$ as yet unknown constants
whereupon the coeffiecents of two different power series are based.
Therefore, the power series solution to (2.0) is

$$
y =
\sum_{m=0}^{\infty} \frac{a_{0}}{m!} x^{2m}
+
\sum_{m=0}^{\infty} \frac{a_{1}}{m!} x^{2m+1}
= a_{0} \exp \left(x^{2}\right) + a_{1} x \exp \left(x^{2}\right)
$$ (2.3)
where $a_{0}$ and $a_{1}$ are constants.

## Problem III

Find a basis of solutions for the following ODE.
Try to identify the series as expansions of known functions.

$$
2 x y^{\prime \prime} + \left(3 - 4x\right) y^{\prime} + \left(2x - 3\right) y = 0
$$ (3.0)

The given ODE can be rewritten as

$$
\left(x - \alpha\right)^{2} A\left(x\right) y^{\prime \prime}
+
\left(x - \alpha\right) B\left(x\right) y^{\prime}
+
C\left(x\right) y = 0,
\quad \alpha = 0,\ A\left(x\right) = \frac{2}{x},\ 
B\left(x\right) = \frac{3-4x}{x},\ C\left(x\right) = 2x-3
$$
$x = \alpha = 0$ is a regular singular point of (3.0).
The indicial equation is

$$
r^{2} + \left[
    \frac{B\left(\alpha\right)}{A\left(\alpha\right)} - 1
\right] r
+ \frac{C\left(\alpha\right)}{A\left(\alpha\right)}
= 0 \quad \Longrightarrow \quad
r^{2} + \frac{1}{2}r = 0
$$ (3.1)
whose roots are $r_{1} = 0$ and $r_{2} = -\frac{1}{2}$.
Since $r_{1} - r_{2} = \frac{1}{2} \notin \mathbb{Z}^{+}$,
we look for two solutions $y_{1}$ and $y_{2}$ of the forms:

$$
y_{1} = x^{r_{1}} \sum_{k=0}^{\infty} a_{k} x^{k}
= \sum_{k=0}^{\infty} a_{k} x^{k}
$$ (3.2a)
$$
y_{2} = x^{r_{2}} \sum_{k=0}^{\infty} b_{k} x^{k}
= x^{-\frac{1}{2}} \sum_{k=0}^{\infty} b_{k} x^{k}
$$ (3.2b)
where $a_{k}$ and $b_{k}$ are constants.

Due to the nature of the roots of (3.1),
$y_{1}$ and $y_{2}$ can be represented by a generic series

$$
y = x^{r} \sum_{k=0}^{\infty} a_{k} x^{k} = \sum_{k=0}^{\infty} a_{k} x^{k+r}
$$ (3.3)
Differentiating with respect to $x$,

$$
y^{\prime} = \sum_{k=0}^{\infty}
\left(k+r\right) a_{k} x^{k+r-1},
\quad
y^{\prime \prime} = \sum_{k=0}^{\infty}
\left(k+r-1\right) \left(k+r\right) a_{k} x^{k+r-2}
$$ (3.4)
Substituting (3.3) and (3.4) onto (3.0) and combining like terms,

$$
\sum_{k=0}^{\infty} \left(2k+2r+1\right) \left(k+r\right) a_{k} x^{k+r-1}
- \sum_{k=0}^{\infty} \left[
    4 \left(k+r\right) + 3
\right] a_{k} x^{k+r}
+ \sum_{k=0}^{\infty} 2 a_{k} x^{k+r+1}
= 0
$$ (3.5a)
Writing down the terms uncommon in all three series,

$$
\left(2r+1\right) ra_{0} x^{r-1} + \left(2r+3\right) \left(r+1\right) a_{1} x^{r}
+ \sum_{k=2}^{\infty} \left(2k+2r+1\right) \left(k+r\right) a_{k} x^{k+r-1}
- \left(4r+3\right) a_{0} x^{r}
- \sum_{k=1}^{\infty} \left[
    4 \left(k+r\right) + 3
\right] a_{k} x^{k+r}
+ \sum_{k=0}^{\infty} 2 a_{k} x^{k+r+1}
= 0
$$ (3.5b)
We can rewrite the three series to be of similar form:

$$
\sum_{k=2}^{\infty} \left(2k+2r+1\right) \left(k+r\right) a_{k} x^{k+r-1}
=
\sum_{n=1}^{\infty} \left[2 \left(n+1\right) + 2r + 1\right]
\left(n+r+1\right) a_{n+1} x^{n+r}
$$
$$
\sum_{k=1}^{\infty} \left[4 \left(k+r\right) + 3\right] a_{k} x^{k+r}
=
\sum_{n=1}^{\infty} \left[4 \left(n+r\right) +3\right] a_{n} x^{n+r}
$$
$$
\sum_{k=0}^{\infty} 2 a_{k} x^{k+r+1}
=
\sum_{n=1}^{\infty} 2 a_{n-1} x^{n+r}
$$
so that the ODE becomes
$$
\left(2r+1\right) ra_{0} x^{r-1} +
\left[
    \left(2r+3\right) \left(r+1\right) a_{1} - \left(4r+3\right) a_{0}
\right] x^{r} +
\sum_{n=1}^{\infty} \left\{
    \left[2\left(n+r\right) + 3\right] \left(n+r+1\right) a_{n+1} -
    \left[4\left(n+r\right) + 3\right] a_{n} +
    2 a_{n-1}
\right\} x^{n+r} = 0
$$ (3.5c)
Owing to homogeneity, the coefficient of any power of $x$ equals zero:

$$
\left(2r+1\right) ra_{0} = 0
$$ (3.6a)
$$
\left(2r+3\right) \left(r+1\right) a_{1} - \left(4r+3\right) a_{0} = 0
\quad \Longrightarrow \quad
a_{1} = \frac{4r+3}{\left(2r+3\right) \left(r+1\right)} a_{0}
$$ (3.6b)
$$
\left[2\left(n+r\right) + 3\right] \left(n+r+1\right) a_{n+1} -
\left[4\left(n+r\right) + 3\right] a_{n} +
2 a_{n-1} = 0
\quad \Longrightarrow \quad
a_{n+1} = \frac{
    \left[4\left(n+r\right) + 3\right] a_{n} - 2 a_{n-1}
}{\left[2\left(n+r\right) + 3\right] \left(n+r+1\right)},
\quad n = 1,2,3,\ldots
$$ (3.6c)
Note that the expression multiplied by $a_{0}$ in (3.6a) is the indicial equation,
*i.e.*, (3.6a) is an identity and $a_{0}$ can be an arbitrary constant.
The recurrence relations (3.6b)-(3.6c) hold for both $r_{1}$ and $r_{2}$.

With $r=r_{1}=0$,

$$
a_{1} = a_{0}; \quad \quad
a_{n+1} = \frac{
    \left[4\left(n+r\right) + 3\right] a_{n} - 2a_{n-1}
}{\left[2\left(n+r\right) + 3\right] \left(n+r+1\right)},
\quad n = 1,2,3,\ldots
$$ (3.7)
where $a_{0}$ is a constant.
Evaluating for a few $n > 1$,

$$
a_{2} = \frac{a_{0}}{2},\quad
a_{3} = \frac{a_{0}}{6},\quad
a_{4} = \frac{a_{0}}{24},\quad
a_{5} = \frac{a_{0}}{120},\quad
a_{6} = \frac{a_{0}}{720}
$$
Hence, the first solution is

$$
y_{1} = \sum_{k=0}^{\infty} a_{k} x^{k}
= a_{0} + a_{0} x + \frac{a_{0}}{2} x^{2} + \frac{a_{0}}{6} x^{3} +
\frac{a_{0}}{24} x^{4} + \frac{a_{0}}{120} x^{5} +
\frac{a_{0}}{720} x^{6} + \cdots
= \sum_{k=0}^{\infty} \frac{a_{0}}{k!} x^{k}
= a_{0} \exp \left(x\right)
$$ (3.8)
where $a_{0}$ is a constant.

With $r=r_{2}=-\frac{1}{2}$, and a harmless substitution of $a$ with $b$,

$$
b_{1} = b_{0}; \quad \quad
b_{n+1} = \frac{
    \left(4n+1\right) b_{n} - 2b_{n-1}
}{\left(n+1\right)\left(2n+1\right)},
\quad n = 1,2,3,\ldots
$$ (3.9)
where $b_{0}$ is a constant. Evaluating for a few $n>1$,

$$
b_{2} = \frac{b_{0}}{2},\quad
b_{3} = \frac{b_{0}}{6},\quad
b_{4} = \frac{b_{0}}{24},\quad
b_{5} = \frac{b_{0}}{120},\quad
b_{6} = \frac{b_{0}}{720}
$$
Hence, the second solution is

$$
y_{2} = x^{-\frac{1}{2}} \sum_{k=0}^{\infty} b_{k} x^{k}
= x^{-\frac{1}{2}} \left[
    b_{0} + b_{0} x + \frac{b_{0}}{2} x^{2} + \frac{b_{0}}{6} x^{3} +
    \frac{b_{0}}{24} x^{4} + \frac{b_{0}}{120} x^{5} +
    \frac{b_{0}}{720} x^{6} + \cdots
\right]
= x^{-\frac{1}{2}} \sum_{k=0}^{\infty} \frac{b_{0}}{k!} x^{k}
= b_{0} x^{-\frac{1}{2}} \exp \left(x\right)
$$ (3.10)
where $b_{0}$ is a constant.

Therefore, since $y_{1}$ and $y_{2}$ are linearly independent,
they constitute a basis of solutions for (3.0).

## Problem IV

Find a basis of solutions for the following ODE.
Try to identify the series as expansions of known functions.

$$
x^{2} y^{\prime \prime} + 2 x^{3} y^{\prime} + \left(x^{2} - 2\right) y = 0
$$ (4.0)

Note that (4.0) can be rewritten as

$$
\left(x - \alpha\right)^{2} A \left(x\right) y^{\prime \prime}
+
\left(x - \alpha\right) B \left(x\right) y^{\prime}
+
C \left(x\right) y
= 0
$$ (4.1)
where $\alpha = 0$, $A \left(x\right) = 1$,
$B \left(x\right) = 2x^{2}$, and
$C \left(x\right) = x^{2} - 2$.
With $A \left(\alpha\right) \neq 0$,
$x = \alpha = 0$ is a regular singular point of (4.0).
The indicial equation would then be

$$
r^{2} +
\left(\frac{B \left(\alpha\right)}{A \left(\alpha\right)} - 1\right) r
+
\frac{C \left(\alpha\right)}{A \left(\alpha\right)}
= 0
\Longrightarrow
r^{2} - r -2 = 0
$$ (4.2)
whose roots are $r_{1} = 2$ and $r_{2} = -1$.
Since $r_{1} - r_{2} = R = 3 \in \mathbb{Z}^{+}$,
we look for two solutions $y_{1}$ and $y_{2}$ of the forms

$$
y_{1} = x^{r_{1}} \sum_{k=0}^{\infty} a_{k} x^{k} = \sum_{k=0}^{\infty} a_{k} x^{k+2}
$$ (4.3a)
$$
y_{2} = c y_{1} \ln x + x^{r_{2}} \sum_{k=0}^{\infty} b_{k} x^{k}
= c y_{1} \ln x + \sum_{k=0}^{\infty} b_{k} x^{k-1}
$$ (4.3b)
where $a_{k}$, $b_{k}$, and $c$ are constants.

We first look for $y_{1}$. Differentiating with respect to $x$,

$$
y_{1}^{\prime} = \sum_{k=0}^{\infty} \left(k+2\right) a_{k} x^{k+1};
\quad
y_{1}^{\prime \prime} = \sum_{k=0}^{\infty} \left(k+1\right) \left(k+2\right) a_{k} x^{k}
$$ (4.4)
Substituting (4.3a) and (4.4) to (4.0), and collecting like terms,

$$
\sum_{k=0}^{\infty} \left[
    \left(k+1\right) \left(k+2\right) - 2
\right] a_{k} x^{k+2}
+
\sum_{k=0}^{\infty} \left(2k+5\right) a_{k} x^{k+4}
= 0
$$ (4.5a)
Explicitly writing the first two terms of the first series
(*i.e.*, $k=0,1$),

$$
0 \cdot a_{0} \cdot x^{2}
+
4 \cdot a_{1} \cdot x^{3}
+
\sum_{k=2}^{\infty} \left[
    \left(k+1\right) \left(k+2\right) - 2
\right] a_{k} x^{k+2}
+
\sum_{k=0}^{\infty} \left(2k+5\right) a_{k} x^{k+4}
= 0
$$ (4.5b)
That the multiplier for $a_{0}$ is $0$ because it is just the indicial equation in disguise.
Because the ODE is homogeneous, the coefficient of each power of $x$ must be zero.
Then, by

$$
0 \cdot a_{0} = 0,
\quad \quad 4 \cdot a_{1} \cdot x^{3} = 0
$$
we deduce that $a_{0}$ must be set by the user and $a_{1} = 0$.
Moreover, we can rewrite the series involving $x^{k+2}$
in terms of $x^{k+4}$ with $k \geq 0$:

$$
\sum_{k=2}^{\infty} \left[
    \left(k+1\right) \left(k+2\right) - 2
\right] a_{k} x^{k+2}
=
\sum_{k=0}^{\infty} \left[
    \left(k+3\right) \left(k+4\right) - 2
\right] a_{k+2} x^{k+4}
$$
Since the terms involving $x^{2}$ and $x^{3}$ are zero,
(4.5b) can now be expressed as a single series in $x^{k+4}$ with $k \geq 0$:

$$
\sum_{k=0}^{\infty} \left\{
    \left[\left(k+3\right) \left(k+4\right) - 2\right] a_{k+2}
    +
    \left(2k + 5\right) a_{k}
\right\} x^{k+4}
= 0
$$ (4.5c)
Due to homogeneity, the coefficient of $x^{k+4}$ must vanish,
giving us a recurrence relation:

$$
a_{k+2} = - \frac{2k + 5}{k^{2} + 7k + 10} a_{k},
\quad k = 0, 1, 2, \ldots
$$ (4.6a)
Having already established that $a_{1} = 0$, we get $a_{k} = 0$ for all odd $k$.
We can thus rewrite (4.6a) to explicitly exclude the odd terms:

$$
a_{2k} = \left(-1\right)^{k} a_{0}
\prod_{j=0}^{k-1} \frac{2j + 5}{j^{2} + 7j + 10},
\quad k = 0, 1, 2, \ldots
$$ (4.6b)
Hence, the first solution $y_{1}$ is

$$
y_{1} = \sum_{k=0}^{\infty} P \left(k\right) a_{0} x^{k+2},
\quad
P \left(k\right) = \left(-1\right)^{k} \prod_{j=0}^{k-1} \frac{2j + 5}{j^{2} + 7j + 10}
$$ (4.7)
where $a_{0}$ is a constant.

Now, from (4.3b),

$$
y_{2} = c y_{1} \ln x + D,
\quad
D = \sum_{k=0}^{\infty} b_{k} x^{k-1}
$$ (4.8a)
$$
y_{2}^{\prime} = c x^{-1} y_{1} + c y_{1}^{\prime} \ln x + D^{\prime},
\quad
D^{\prime} = \sum_{k=0}^{\infty} \left(k-1\right) b_{k} x^{k-2}
$$ (4.8b)
$$
y_{2}^{\prime \prime} = -c x^{-2} y_{1} + 2c x^{-1} y_{1}^{\prime} + c y_{1}^{\prime \prime} \ln x + D^{\prime \prime},
\quad
D^{\prime \prime} = \sum_{k=0}^{\infty} \left(k-1\right) \left(k-2\right) b_{k} x^{k-3}
$$ (4.8c)
Substituting (4.8) to (4.0),

$$
-cy_{1} + 2cxy_{1} + cx^{2} y_{1}^{\prime \prime} \ln x + x^{2} D^{\prime \prime}
+ 2cx^{2} y_{1} + 2cx^{3} y_{1}^{\prime} \ln x + 2x^{3} D^{\prime}
+ \left(x^{2} - 2\right) cy_{1} \ln x + \left(x^{2} - 2\right) D = 0
$$ (4.9a)
Rearranging the ugly mess that is (4.9a),

$$
\left(2x^{2}-1\right) cy_{1} + 2cxy_{1}^{\prime}
+
\left[
    x^{2} y_{1}^{\prime \prime} + 2x^{3} y_{1}^{\prime} + \left(x^{2} - 2\right) y_{1}
\right] c \ln x
+
\left[
    x^{2} D^{\prime \prime} + 2x^{3} D^{\prime} + \left(x^{2} - 2\right) D
\right]
= 0
$$ (4.9b)
Observe that the quantity inside the first bracket in (4.9b)
is just applying $y_{1}$ onto (4.0)&mdash;it is equal to zero:

$$
\left(2x^{2}-1\right) cy_{1} + 2cxy_{1}^{\prime} +
\left[
    x^{2} D^{\prime \prime} + 2x^{3} D^{\prime} + \left(x^{2} - 2\right) D
\right] = 0
$$ (4.9c)
We can rewrite (4.9c) as a "matching" of series:

$$
x^{2} D^{\prime \prime} + 2x^{3} D^{\prime} + \left(x^{2} - 2\right) D
= -2cxy_{1}^{\prime} + \left(1 - 2x^{2}\right) cy_{1}
$$ (4.10)
Using the definitions for $D$ and its derivatives in (4.8),
we can list out the first few terms in the left hand side of (4.10):

$$
0\cdot b_{0} x^{-1} - 2b_{1} x^{0} - \left(2b_{2} - b_{0}\right) x^{1}
+ \left(0\cdot b_{3} + b_{1}\right) x^{2} + \cdots
$$ (4.11)
In series form, the right hand side of (4.10) is

$$
- \sum_{k=0}^{\infty} c\left(2k+3\right) P\left(k\right) a_{0} x^{k+2}
- \sum_{k=0}^{\infty} 2c P\left(k\right) a_{0} x^{k+4}
=
- 3 ca_{0} x^{2} + \frac{5}{2} ca_{0} x^{3} + \cdots
$$ (4.12)
Comparing the $x^{-1}$ and $x^{0}$ terms in (4.11) and (4.12),
we can deduce information for $b_{0}$ and $b_{1}$:

- $0\cdot b_{0} = 0$ suggests that $b_{0}$ is a constant to be set by the user.
- $-2b_{1} = 0$ means $b_{1} = 0$.
- $-2b_{2} - b_{0} = 0$ means $b_{2} = -\frac{1}{2} b_{0}$.

Comparing the $x^{2}$ terms in (4.11) and (4.12),

$$
0\cdot b_{3} + b_{1} = -3ca_{0} \Longrightarrow ca_{0} = 0
$$ (4.13)
which means that we can set $c=0$ regardless of $a_{0}$.
As such $y_{2}$ is rid of the logarithm term:

$$
y_{2} = \sum_{k=0}^{\infty} b_{k} x^{k-1}
= b_{0} x^{-1} + b_{1} + b_{2} x^{1} +
b_{3} x^{2} + b_{4} x^{3} + b_{5} x^{4} + \cdots
$$
Moreover, notice that
$b_{3} x^{2} + b_{4} x^{3} + b_{5} x^{4} + \cdots$
is just a linear transformation of
$y_{1} = P_{0} a_{0} x^{2} + P_{1} a_{1} x^{3} + P_{2} a_{2} x^{4} + \cdots$,
and hence must be excluded from being a distinct solution.
The second solution now reduces to a polynomial

$$
y_{2} = b_{0} x^{-1} + b_{1} + b_{2} x^{1}
$$
Differentiating $y_{2}$ with respect to $x$,

$$
y_{2}^{\prime}= -b_{0} x^{-2} + b_{2},
\quad
y_{2}^{\prime \prime} = 2b_{0} x^{-3}
$$
and substituting onto (4.0) yields

$$
-\left(b_{0} + 2b_{2}\right) x + b_{1} x^{2} + 3b_{2} x^{3} - 2b_{1} = 0
$$
whence we derive the same information earlier presented in (4.12), namely
$b_{1} = 0$ and $b_{2} = -\frac{1}{2} b_{0}$.
We also know from the $x^{3}$ term that $b_{2} = 0$, and thus $b_{0} = 0$.
The second solution, after all the analyses, turns out to be trivial:

$$
y_{2} = 0
$$ (4.14)
Therefore, the basis of solutions to (4.0) consists of
a non-trivial Frobenius series $y_{1}$
and a trivial $y_{2} = 0$:

$$
y = y_{1} + y_{2} =
\sum_{k=0}^{\infty} P \left(k\right) a_{0} x^{k+2},
\quad
P \left(k\right) = \left(-1\right)^{k} \prod_{j=0}^{k-1} \frac{2j + 5}{j^{2} + 7j + 10}
$$ (4.15)
where $a_{0}$ is a constant.

## Problem V

Find the general solution
(in terms of $J_{\textsf{v}}$ and $Y_{\textsf{v}}$)
to the following ODE
by using $12 \sqrt{x} = z$:

$$
x y^{\prime \prime} + y^{\prime} + 36y = 0
$$ (5.0)

For some quantities $a$ and $b$,
let $a_{b}$ and $a_{bb}$ denote the first and second derivatives of $a$ with respect to $b$,
respectively, assuming that such derivatives exist.
From the given substitution scheme:

$$
z = 12 \sqrt{x}
\quad \Longrightarrow \quad
z_{x} = 6 x^{-\frac{1}{2}}
\quad \Longrightarrow \quad
z_{xx} = -3 x^{-\frac{3}{2}}
$$ (5.1)
Assume that $y$ is a composition of $z$ and $x$, so that by the chain rule,

$$
y^{\prime} = y_{x} = y_{z} z_{x} = 6 x^{-\frac{1}{2}} y_{z}
\quad \Longrightarrow \quad
y^{\prime \prime} = y_{z} z_{xx} + \left(z_{x}\right)^{2} y_{zz}
= -3x^{\frac{3}{2}} y_{z} + 6x^{-1} y_{zz}
$$ (5.2)
Substituting (5.2) to (5.0),

$$
x \left[-3x^{\frac{3}{2}} y_{z} + 6x^{-1} y_{zz}\right]
+ 6x^{-\frac{1}{2}} y_{z} + 36y = 0
\quad \Longrightarrow \quad
12x^{\frac{1}{2}} y_{zz} + y_{z} + 12x^{\frac{1}{2}} y = 0
$$
and invoking the substitution scheme,

$$
z y_{zz} + y_{z} + zy = 0
\quad \Longrightarrow \quad
z^{2} y_{zz} + z y_{z} + \left(z^{2} - \nu^{2}\right) y = 0,
\quad \nu = 0
$$ (5.3)

In other words, the transformation $z = 12\sqrt{x}$
allows the reformulation of an Euler-Cauchy ODE (5.0)
into a Bessel equation of order $\nu = 0$.
This eventually leads to two solutions
$J_{0} \left(z\right)$ and $Y_{0} \left(z\right)$.
The first solution is a Bessel function of the first kind of order zero:

$$
J_{0} \left(z\right) = \sum_{k=0}^{\infty}
\frac{\left(-1\right)^{k}}{
    2^{2k} \left[\Gamma \left(k+1\right)\right]^{2}
} z^{2k}
= \sum_{k=0}^{\infty}
\frac{\left(-1\right)^{k}}{
    2^{2k} \left(k!\right)^{2}
} z^{2k}
$$ (5.4a)
The second solution is a Bessel function of the second kind of order zero:

$$
Y_{0} \left(z\right) = \frac{2}{\pi}
\left[
    \left(\ln \frac{z}{2} + \gamma \right) J_{0} \left(z\right) +
    \sum_{k=0}^{\infty} \frac{
        \left(-1\right)^{k} H \left(k+1\right)
    }{
        2^{2k} \left(k!\right)^{2}
    }z^{2k}
\right]
$$ (5.4b)
where $\gamma$ is the Euler-Mascheroni constant
and $H \left(k\right)$ is the harmonic series:

$$
\gamma = \lim_{n \rightarrow +\infty}
\left(-\ln n + \sum_{k=1}^{n} \frac{1}{k} \right)
\approx 0.57722, \quad
H \left(k\right) = 1 + \frac{1}{2} + \frac{1}{3}
+ \cdots + \frac{1}{k}
$$ (5.4c)
The general solution to the Bessel equation (5.3) is

$$
y \left(z\right) = C_{J} J_{0} \left(z\right) + C_{Y} Y_{0} \left(z\right)
$$
where $C_{J}$ and $C_{Y}$ are constants.
Expressing back in terms of $x$ by substituting $z = 12\sqrt{x}$,
the general solution to the given Euler-Cauchy ODE (5.0) is

$$
J_{0} \left(x\right) = \sum_{k=0}^{\infty}
\frac{\left(-144\right)^{k}}{
    2^{2k} \left(k!\right)^{2}
} x^{k}
$$ (5.5a)
$$
Y_{0} \left(x\right) = \frac{2}{\pi}
\left[
    \left(\ln \frac{z}{2} + \gamma \right) J_{0} \left(x\right) +
    \sum_{k=0}^{\infty} \frac{
        \left(-144\right)^{k} H \left(k+1\right)
    }{
        2^{2k} \left(k!\right)^{2}
    }x^{k}
\right]
$$ (5.5b)
$$
y \left(x\right) = C_{J} J_{0} \left(x\right) + C_{Y} Y_{0} \left(x\right)
$$ (5.5c)
where $C_{J}$ and $C_{Y}$ are constants.
