# Answers to Problem Set III

*Prepared by*
Christian Y. Cahig

# Problem I

Find the general solution to the following ODE:

$$
y^{\prime \prime}
-
144y
=
0
$$ (1.0)

Following Kreyzsig's convention,
the given ODE can be rewritten as
$y^{\prime \prime} + \alpha y^{\prime} + \beta y = 0$
where
$\alpha = 0$
and
$\beta = -144$.
The characteristic equation (in $\lambda$) is then

$$
\lambda^{2} + \alpha \lambda + \beta = 0
\quad \Longrightarrow \quad
\lambda^{2} - 144 = 0
$$ (1.1)
whose roots are
$\lambda_1 = + 12$
and
$\lambda_2 = - 12$.
This means that there are two basis functions
comprising the general solution,
*i.e.*,
$e^{12x}$
and
$e^{-12x}$.
Hence, the general solution to (1.0) is

$$
y = C_1 e^{12x} + C_2 e^{-12x}
$$ (1.2)
where $C_1$ and $C_2$ are constants.

# Problem II

Find the general solution to the following ODE:

$$
4 y^{\prime \prime}
-
20 y^{\prime}
+
25 y
=
0
$$ (2.0)

Dividing both sides of (2.0) by 4,
we get the equivalent standard form
(at least, according to Kreyzsig's convention)

$$
y^{\prime \prime}
-
5 y^{\prime}
+
\frac{25}{4} y
=
0
$$ (2.1)
where
$\alpha = -5$
and
$\beta = \frac{25}{4}$.
Then, the characteristic equation (in $\lambda$) is

$$
\lambda^{2} + \alpha \lambda + \beta = 0
\quad \Longrightarrow \quad
\lambda^2 -5 \lambda + \frac{25}{4} = 0
$$ (2.2)

Notice that (2.2) is a perfect square binomial:

$$
\lambda^{2}
-
2 \left(\frac{5}{2}\right) y
+
\left(\frac{5}{2}\right)^{2}
=
0
\quad \Longrightarrow \quad
\left(\lambda - \frac{5}{2}\right) = 0
$$
In other words,
the charateristic equation
has a real root of 2.5
with multiplicity of 2.
This means that the general solution
has two basis functions:
$e^{2.5x}$
and
$x e^{2.5x}$.
Hence, the general solution to (2.0) is

$$
y
=
\left(C_1 + C_2 x\right)
e^{2.5x}
$$ (2.3)
where $C_1$ and $C_2$ are constants.

# Problem III

Find the particular solution to the following ODE:

$$
y^{\prime \prime}
+
4 y^{\prime}
+
5 y
=
0,
\quad
y \left(0\right) = 2,
\quad
y^{\prime} \left(0\right) = -5
$$ (3.0)

From Kreyzsig's convention,
the given ODE is of the standard form with
$\alpha = 4$
and
$\beta = 5$.
The characteristic equation (in $\lambda$) is then

$$
\lambda^2 + \alpha \lambda + \beta = 0
\quad \Longrightarrow \quad
\lambda^2 + 4 \lambda + 5 = 0
$$ (3.1)

By the quadratic formula,
the roots of (3.1) are
$\lambda_1 = - 2 + i$
and
$\lambda_2 = - 2 - i$.
Then, the basis functions
that make up the general solution
to (3.0) are
$e^{-2x} \cos x$
and
$e^{-2x} \sin x$.
Hence, the general solution to (3.0) is

$$
y
=
e^{-2x}
\left(C_1 \cos x + C_2 \sin x\right)
$$ (3.2)
where $C_1$ and $C_2$ are constants.

Knowing that $y \left(0\right) = 2$,

$$
e^{-2 \left(0\right)}
\left[
C_1 \cos (0)
+
C_2 \sin (0)
\right]
= 2
\quad \Longrightarrow \quad
C_1 = 2
$$ (3.3)
Differentiating both sides of (3.2)
with respect to $x$,

$$
y^{\prime} =
e^{-2x}
\left[
\left(-2 C_1 + C_2\right) \cos x
-
\left(C_1 + 2 C_2\right) \sin x
\right]
$$
substituting (3.3) onto (3.2),
differentiating $y$ with respect to $x$,
and
invoking $y^{\prime} \left(0\right) = -5$,

$$
e^{-2 \left(0\right)}
\left[
\left(-4 + C_2\right) \cos \left(0\right)
-
\left(2 + 2 C_2\right) \sin \left(0\right)
\right]
= -5
\quad \Longrightarrow \quad
C_2 = -1
$$ (3.4)

Hence, the particular solution to (3.0) is

$$
y = e^{-2x}
\left(2 \cos x - \sin x\right)
$$ (3.5)

# Problem IV

Find the general solution to the following ODE:

$$
\left(D^{2} -6D + 13I\right) y = 0
$$ (4.0)

Assuming that
$D$ denotes differentiating with respect to $x$
and
$I$ denotes the identity operator,
can be rewritten as
$y^{\prime \prime} + \alpha y^{\prime} + \beta y = 0$
where
$\alpha = -6$
and
$\beta = 13$.
The corresponding characteristic equation
(in $\lambda$) is

$$
\lambda^2 - 6 \lambda + 13 = 0
$$ (4.1)
whose roots are
$\lambda_1 = 3 + 2i$
and
$\lambda_2 = 3 - 2i$.
This leads to two basis functions
$e^{3x} \cos \left(2x\right)$
and
$e^{3x} \sin \left(2x\right)$
making up the general solution,
*i.e.*,

$$
y = e^{3x}
\left[
C_1 \cos \left(2x\right)
+
C_2 \sin \left(2x\right)
\right]
$$ (4.2)
where $C_1$ and $C_2$ are constants.

# Problem V

Find the particular solution to the following ODE:

$$
x^2 y^{\prime \prime}
-
4 x y^{\prime}
+
6 y
=
0,
\quad
y \left(1\right) = 1,
\quad
y^{\prime} \left(1\right) = 0
$$ (5.0)

By Kreyzig's convention,
(5.0) is an Euler-Cauchy equation
of the form
$x^2 y^{\prime \prime} + \alpha x y^{\prime} + \beta y = 0$
where
$\alpha = -4$
and
$\beta = 6$.
This leads to an auxiliary equation
(in $\lambda$) of

$$
\lambda^2 + \left(\alpha - 1\right) + \beta = 0
\quad \Longrightarrow \quad
\lambda^2 - 5 \lambda + 6 = 0
$$ (5.1)
whose roots are
$\lambda_1 = 2$
and
$\lambda_2 = 3$.
This eventually leads to a general solution of

$$
y = C_1 x^{\lambda_1} + C_2 x^{\lambda_2}
\quad \Longrightarrow \quad
y = C_1 x^2 + C_2 x^3
$$ (5.2)
where $C_1$ and $C_2$ are constants.

Knowing that $y \left(1\right) = 1$,

$$
C_1 \left(1\right)^{2} + C_2 \left(1\right)^{3} = 1
\quad \Longrightarrow \quad
C_1 + C_2 = 1
$$ (5.3)
Differentiating both sides of (5.2) with respect to $x$
and invoking $y^{\prime} \left(1\right) = 0$,

$$
2 C_1 \left(1\right) + 3 C_2 \left(1\right)^{2} = 0
\quad \Longrightarrow \quad
2 C_1 + 3 C_2 = 0
$$ (5.4)
From (5.3) and (5.4),
$C_1 = 3$
and
$C_2 = -2$.
Hence, the particular solution to (5.0) is

$$
y = 3 x^2 - 2 x^3
$$ (5.5)

# Problem VI

Find the general solution to the following ODE
using the
Method of Undetermined Coefficients:

$$
\left(D^2 - 4\right) y
=
4x - 3 e^{x}
$$ (6.0)

Neglecting the right hand side of (6.0),
the "homogenized" ODE will lead to a characteristic equation
with roots $\plusmn 2$.
The homogeneous solution $y_{\textsf{h}}$ is then

$$
y_{\textsf{h}}
=
C_1 e^{2x} + C_2 e^{-2x}
$$ (6.1)
where $C_1$ and $C_2$ are constants.

By inspecting the right hand side of (6.0),
we can deduce&ndash;of course by principled intuition&ndash;that
the particular solution $y_{\textsf{p}}$
is of the form

$$
y_{\textsf{p}} =
\alpha_1 x + \alpha_0 + \beta e^x
$$ (6.2)
where the $\alpha$ and $\beta$ terms are are constants.
Differentating both sides of (6.2)
twice with respect to $x$
will give
$y_{\textsf{p}}^{\prime \prime} = \beta e^x$.
Substituting
$y_{\textsf{p}}$
and
$y_{\textsf{p}}^{\prime \prime}$
onto (6.0),

$$
y_{\textsf{p}}^{\prime \prime} - 4 y_{\textsf{p}} = 4x - 3e^{x}
\quad \Longrightarrow \quad
-4 \alpha_1 x - 3 \beta e^x - 4 \alpha_0
=
4x - 3e^x
\quad \Longrightarrow \quad
\alpha_1 = -1,\ \alpha_0 = 0,\ \beta = 1
$$
The particular solution is then

$$
y_{\textsf{p}} =
e^x - x
$$ (6.3)

Hence, the general solution to (6.0) is the superposition
of $y_{\textsf{h}}$ and $y_{\textsf{p}}$:

$$
y
= y_{\textsf{h}} + y_{\textsf{p}}
= C_1 e^{2x} + C_2 e^{-2x} + e^x - x
$$ (6.4)
where $C_1$ and $C_2$ are constants.

# Problem VII

Find the general solution to the following ODE
using the
Method of Variation of Parameters:

$$
\left(D^2 - 4\right) y
=
4x - 3 e^{x}
$$ (7.0)

Note that the corresponding homogeneous ODE of (7.0)
has a characteristic equation
with roots $\plusmn 2$.
The homogeneous solution $y_{\textsf{h}}$
is then made up of two basis functions
$e^{2x}$ and $e^{-2x}$:

$$
y_{\textsf{h}}
=
C_1 e^{2x} + C_2 e^{-2x}
$$ (7.1)
where $C_1$ and $C_2$ are constants.

By Lagrange's method, the particular solution is

$$
y_{\textsf{p}}
=
- e^{2x} \int \frac{e^{-2x} R\left(x\right)}{W\left(x\right)} dx
+ e^{-2x} \int \frac{e^{2x} R\left(x\right)}{W\left(x\right)} dx
$$
where
$R \left(x\right) = 4x - 3 e^x$ 
is the right hand side of (7.0)
and 
$W \left(x\right)$ is the Wronskian of the basis functions
given as

$$
W\left(x\right) =
e^{2x} \frac{d}{dx} \left(e^{-2x}\right)
-
e^{-2x} \frac{d}{dx} \left(e^{2x}\right)
=
-4
$$
Expressing $y_{\textsf{p}}$ fully,

$$
y_{\textsf{p}}
=
-
e^{2x} \int \frac{e^{-2x} \left(4x - 3 e^x\right)}{-4} dx
+
e^{-2x} \int \frac{e^{2x} \left(4x - 3 e^x\right)}{-4} dx
\ \ \ \ \ \ \ \ \ \ \ \ \ \ \ \ \ \ \ \ \ \ \ \ \ 
$$

$$
=
e^{2x} \int \left(x e^{-2x} - \frac{3}{4} e^{-x}\right) dx
-
e^{-2x} \int \left(x e^{2x} - \frac{3}{4} e^{3x}\right) dx
\ \ \ \ \ \ \ \ \ \ \ \ \ \ \ \ \ \ \ 
$$

$$
=
e^{2x} \int x e^{-2x} dx
-
\frac{3}{4} e^{2x} \int e^{-x} dx
-
e^{-2x} \int x e^{2x} dx
+
\frac{3}{4} e^{-2x} \int e^{3x} dx
$$
Evaluating the terms with the simpler integrals
involving $e^{-x}$ and $e^{3x}$:

$$
-
\frac{3}{4} e^{2x} \int e^{-x} dx
+
\frac{3}{4} e^{-2x} \int e^{3x} dx
=
\frac{3}{4} e^{2x} e^{-x}
+
\frac{1}{4} e^{-2x} e^{3x}
=
e^{x}
$$ (7.2a)
We can evaluate the integral involving $x e^{-2x}$
by decomposing the differential into
two parts
$u = x$
and
$dv = e^{-2x} dx$,
so that

$$
e^{2x} \int x e^{-2x} dx
=
e^{2x}
\left(
- \frac{1}{2} x e^{-2x}
+ \int \frac{1}{2} e^{-2x} dx
\right)
=
e^{2x}
\left(
- \frac{1}{2} x e^{-2x}
- \frac{1}{4} e^{-2x}
\right)
=
\frac{-2x - 1}{4}
$$ (7.2b)
For the integral involving $x e^{2x}$
we decompose the differential into
two parts
$u = x$
and
$dv = e^{2x} dx$,
so that

$$
- e^{-2x} \int x e^{2x} dx
=
- e^{-2x}
\left(
\frac{1}{2} x e^{2x}
-
\int \frac{1}{2} e^{2x} dx
\right)
=
- e^{-2x}
\left(
\frac{1}{2} x e^{2x}
- \frac{1}{4} e^{2x}
\right)
=
\frac{-2x + 1}{4}
$$ (7.2c)
The particular solution is
then the sum of the results in (7.2a)-(7.2c):

$$
y_{\textsf{p}}
=
e^x + \frac{-2x - 1}{4} + \frac{-2x + 1}{4}
=
e^x - x
$$ (7.3)

Finally, the general solution to (7.0)
is the superposition of
$y_{\textsf{h}}$ and $y_{\textsf{p}}$:

$$
y
= y_{\textsf{h}} + y_{\textsf{p}}
= C_1 e^{2x} + C_2 e^{-2x} + e^x - x
$$ (7.4)
where $C_1$ and $C_2$ are constants.
